feat: inferConstant.WF, environment proofs

Lean4Lean/Theory/VEnv.lean
@@ -31,12 +31,12 @@ def VEnv.addDefEq (env : VEnv) (df : VDefEq) : VEnv :=
   { env with defeqs := fun x => x = df ∨ env.defeqs x }
 
 structure VEnv.LE (env1 env2 : VEnv) : Prop where
-  constants (n a) : env1.constants n = some a → env2.constants n = some a
-  defeqs (df) : env1.defeqs df → env2.defeqs df
+  constants : env1.constants n = some a → env2.constants n = some a
+  defeqs : env1.defeqs df → env2.defeqs df
 
 instance : LE VEnv := ⟨VEnv.LE⟩
 
-theorem VEnv.LE.rfl {env : VEnv} : env ≤ env := ⟨fun _ _ => id, fun _ => id⟩
+theorem VEnv.LE.rfl {env : VEnv} : env ≤ env := ⟨id, id⟩
 
 theorem VEnv.LE.trans {a b c : VEnv} (h1 : a ≤ b) (h2 : b ≤ c) : a ≤ c :=
-  ⟨fun _ _ => h2.1 _ _ ∘ h1.1 _ _, fun _ => h2.2 _ ∘ h1.2 _⟩
+  ⟨h2.1 ∘ h1.1, h2.2 ∘ h1.2⟩
