Lean4Lean/Verify/Environment.lean
@@ -24,21 +24,37 @@ def TrDefVal (ci : ConstantInfo) (ci' : VDefVal) : Prop :=
   TrConstVal safety env ci ci'.toVConstVal ∧
   TrExprS env ci.levelParams [] ci.value! ci'.value
 
-def AddQuot1 (env : VEnv) (name : Name) (kind : QuotKind) (ci' : VConstant) (P : ConstMap → Prop)
-    (m : ConstMap) : Prop :=
-  ∃ levelParams type,
+def AddQuot1 (name : Name) (kind : QuotKind) (ci' : VConstant) (P : ConstMap → VEnv → Prop)
+    (m : ConstMap) (env : VEnv) : Prop :=
+  ∃ levelParams type env',
     let ci := .quotInfo { name, kind, levelParams, type }
     TrConstant .safe env ci ci' ∧
-    P (m.insert name ci)
+    env.addConst name ci' = some env' ∧
+    P (m.insert name ci) env'
 
-def AddQuot (env : VEnv) (m1 m2 : ConstMap) : Prop :=
-  AddQuot1 env ``Quot .type quotConst (m := m1) <|
-  AddQuot1 env ``Quot.mk .ctor quotMkConst <|
-  AddQuot1 env ``Quot.lift .lift quotLiftConst <|
-  AddQuot1 env ``Quot.ind .ind quotMkConst (Eq m2)
+theorem AddQuot1.to_addQuot
+    (H1 : ∀ m env, P m env → f env = some env')
+    (m env) (H : AddQuot1 name kind ci' P m env) :
+    env.addConst name (some ci') >>= f = some env' := by
+  let ⟨_, _, _, h1, h2, h3⟩ := H
+  simpa using ⟨_, h2, H1 _ _ h3⟩
 
-inductive AddInduct (m1 : ConstMap) (decl : VInductDecl) (m2 : ConstMap) : Prop
+def AddQuot (m₁ m₂ : ConstMap) (env₁ env₂ : VEnv) : Prop :=
+  AddQuot1 ``Quot .type quotConst (m := m₁) (env := env₁) <|
+  AddQuot1 ``Quot.mk .ctor quotMkConst <|
+  AddQuot1 ``Quot.lift .lift quotLiftConst <|
+  AddQuot1 ``Quot.ind .ind quotIndConst (· = m₂ ∧ ·.addDefEq quotDefEq = env₂)
+
+nonrec theorem AddQuot.to_addQuot (H : AddQuot m₁ m₂ env₁ env₂) : env₁.addQuot = some env₂ :=
+  open AddQuot1 in (to_addQuot <| to_addQuot <| to_addQuot <| to_addQuot (by simp)) _ _ H
+
+inductive AddInduct (m₁ : ConstMap) (env₁ : VEnv) (decl : VInductDecl)
+    (m₂ : ConstMap) (env₂ : VEnv) : Prop
   -- TODO
+
+nonrec theorem AddInduct.to_addInduct
+    (H : AddInduct m₁ env₁ decl m₂ env₂) : env₁.addInduct decl = some env₂ :=
+  nomatch H
 
 variable (safety : DefinitionSafety) in
 inductive TrEnv' : ConstMap → Bool → VEnv → Prop where
@@ -68,21 +84,19 @@ inductive TrEnv' : ConstMap → Bool → VEnv → Prop where
     TrEnv' (C.insert ci.name (.opaqueInfo ci)) Q env'
   | quot :
     env.QuotReady →
-    env.addQuot = some env' →
-    AddQuot env C C' →
+    AddQuot C C' env env' →
     TrEnv' C false env →
     TrEnv' C' true env'
   | induct :
     decl.WF env →
-    env.addInduct decl = some env' →
-    AddInduct C decl C' →
+    AddInduct C env decl C' env' →
     TrEnv' C Q env →
     TrEnv' C' Q env'
 
 def TrEnv (safety : DefinitionSafety) (env : Environment) (venv : VEnv) : Prop :=
   TrEnv' safety env.constants env.quotInit venv
 
-theorem TrEnv'.WF (H : TrEnv' C Q env venv) : venv.WF := by
+theorem TrEnv'.wf (H : TrEnv' safety C Q venv) : venv.WF := by
   induction H with
   | empty => exact ⟨_, .empty⟩
   | block _ h _ ih =>
@@ -99,11 +113,9 @@ theorem TrEnv'.WF (H : TrEnv' C Q env venv) : venv.WF := by
     have ⟨_, H⟩ := ih
     have := h1.1.2; dsimp [ConstantInfo.name, ConstantInfo.toConstantVal] at this
     exact ⟨_, H.decl <| .opaque h2 (this ▸ h3)⟩
-  | quot h1 h2 _ _ ih =>
+  | quot h1 h2 _ ih =>
     have ⟨_, H⟩ := ih
-    exact ⟨_, H.decl <| .quot h1 h2⟩
-  | induct h1 h2 _ _ ih =>
+    exact ⟨_, H.decl <| .quot h1 h2.to_addQuot⟩
+  | induct h1 h2 _ ih =>
     have ⟨_, H⟩ := ih
-    exact ⟨_, H.decl <| .induct h1 h2⟩
-
-nonrec theorem TrEnv.WF (H : TrEnv safety env venv) : venv.WF := H.WF
+    exact ⟨_, H.decl <| .induct h1 h2.to_addInduct⟩
