Lean4Lean/Std/HashMap.lean
@@ -1,0 +1,99 @@
+import Std.Data.HashMap.Lemmas
+import Lean
+
+namespace Std.Internal.List
+
+namespace Const
+
+def containsKey [BEq α] (a : α) : List (α × β) → Bool
+  | [] => false
+  | ⟨k, _⟩ :: l => k == a || containsKey a l
+
+def replaceEntry [BEq α] (k : α) (v : β) : List (α × β) → List (α × β)
+  | [] => []
+  | ⟨k', v'⟩ :: l => bif k' == k then ⟨k, v⟩ :: l else ⟨k', v'⟩ :: replaceEntry k v l
+
+def insertEntry [BEq α] (k : α) (v : β) (l : List (α × β)) : List (α × β) :=
+  bif containsKey k l then replaceEntry k v l else (k, v) :: l
+
+theorem insertEntry_perm_filter [BEq α] [PartialEquivBEq α]
+    (k : α) (v : β) {l : List (α × β)} (hl : l.Pairwise (fun a b => (a.1 == b.1) = false)) :
+    (insertEntry k v l).Perm <| (k, v) :: l.filter (¬k == ·.1) := by
+  unfold insertEntry
+  cases eq : containsKey k l <;> simp
+  · rw [List.filter_eq_self.2]
+    induction l <;> simp_all [containsKey, BEq.comm]; assumption
+  · induction l <;> simp_all [-List.pairwise_cons, containsKey, replaceEntry, List.filter, BEq.comm]
+    revert eq; cases h : k == _ <;> intro eq <;> simp_all
+    rename_i ih
+    · exact .trans (.cons _ ih) (.swap ..)
+    · rw [List.filter_eq_self.2]
+      intro ⟨a, b⟩ h'
+      have := hl.1 a b h'
+      refine Decidable.by_contra fun h2 => ?_
+      simp at h2
+      cases h2.symm.trans (BEq.congr_left h ▸ this)
+
+end Const
+
+theorem containsKey_map [BEq α] (l : List ((_ : α) × β)) :
+    Const.containsKey k (l.map (fun x => (x.1, x.2))) = containsKey k l := by
+  induction l <;> simp [containsKey, Const.containsKey, *]
+
+theorem replaceEntry_map [BEq α] (l : List ((_ : α) × β)) :
+    Const.replaceEntry k v (l.map (fun x => (x.1, x.2))) =
+    (replaceEntry k v l).map (fun x => (x.1, x.2)) := by
+  induction l <;> simp [replaceEntry, Const.replaceEntry, *]
+  cases _ == k <;> simp
+
+theorem insertEntry_map [BEq α] (l : List ((_ : α) × β)) :
+    Const.insertEntry k v (l.map (fun x => (x.1, x.2))) =
+    (insertEntry k v l).map (fun x => (x.1, x.2)) := by
+  simp [insertEntry, Const.insertEntry, containsKey_map, replaceEntry_map]
+  cases containsKey k l <;> simp
+
+end Std.Internal.List
+
+namespace Std.DHashMap
+open Std.Internal.List Internal.Raw Internal.Raw₀
+
+variable [BEq α] [Hashable α] [EquivBEq α] [LawfulHashable α]
+
+theorem insert_perm_insertEntry (m : DHashMap α β) (a b) :
+    (insert m a b).toList.Perm (insertEntry a b m.toList) := by
+  simp [toList, toList_eq_toListModel]
+  exact toListModel_insert (WF.out m.2)
+
+theorem Const.insert_perm_insertEntry (m : DHashMap α fun _ => β) (a b) :
+    (Const.toList (insert m a b)).Perm (Const.insertEntry a b (Const.toList m)) := by
+  simp [Const.toList, Const.toList_eq_toListModel_map, insertEntry_map]
+  exact (toListModel_insert (WF.out m.2)).map _
+
+end Std.DHashMap
+
+namespace Std.HashMap
+open Internal.List
+
+variable [BEq α] [Hashable α] [LawfulHashable α]
+
+theorem insert_toList [EquivBEq α] (m : HashMap α β) :
+    (insert m a b).toList.Perm ((a, b) :: m.toList.filter (¬a == ·.1)) := by
+  refine (DHashMap.Const.insert_perm_insertEntry m.1 a b).trans ?_
+  exact Const.insertEntry_perm_filter _ _ distinct_keys_toList
+
+theorem getElem?_eq_lookup_toList [LawfulBEq α] (m : HashMap α β) (a : α) :
+    m[a]? = m.toList.lookup a := by
+  apply Option.ext fun b => ?_
+  simp; rw [← mem_toList_iff_getElem?_eq_some]
+  have := distinct_keys_toList (m := m); revert this
+  induction m.toList <;> intro H <;> simp_all [List.lookup]
+  split <;> simp_all [Prod.ext_iff]
+  simp [eq_comm]
+  rw [List.lookup_eq_none_iff.2]; · simp
+  simp; exact H.1
+
+theorem mem_of_getElem? [EquivBEq α] {m : HashMap α β} (h : m[a]? = some b) : a ∈ m := by
+  refine Decidable.by_contra fun h' => ?_
+  cases (getElem?_eq_none h').symm.trans h
+
+end Std.HashMap
