Lean4Lean/Std/PersistentHashMap.lean
@@ -1,0 +1,42 @@
+import Lean.Data.SMap
+import Std.Data.HashMap.Lemmas
+import Lean4Lean.Verify.Axioms
+
+namespace Lean.PersistentHashMap
+
+@[simp] theorem toList'_empty [BEq α] [Hashable α] :
+    (.empty : PersistentHashMap α β).toList' = [] := by
+  have this n : @Node.toList' α β (.entries ⟨.replicate n .null⟩) = [] := by
+    simp [Node.toList']
+    induction n <;> simp [*, List.replicate_succ]
+  apply this
+
+@[simp] theorem toList'_empty' [BEq α] [Hashable α] :
+    ({} : PersistentHashMap α β).toList' = [] := toList'_empty
+
+theorem find?_isSome {α β} [BEq α] [Hashable α]
+    (m : PersistentHashMap α β) (a : α) : m.contains a = (m.find? a).isSome := findAux_isSome ..
+
+theorem WF.nodupKeys [BEq α] [Hashable α]
+    [LawfulBEq α] [LawfulHashable α]
+    {m : PersistentHashMap α β} (h : WF m) : m.toList'.NodupKeys := by
+  induction h with
+  | empty => simp; exact .nil
+  | insert h1 ih =>
+    refine (h1.toList'_insert ..).nodupKeys_iff.2 (List.nodupKeys_cons.2 ⟨?_, ih.filter _⟩)
+    rintro _ h3 rfl
+    simpa using (List.mem_filter.1 h3).2
+
+variable [BEq α] [LawfulBEq α] [Hashable α] [LawfulHashable α] in
+theorem WF.find?_insert {s : PersistentHashMap α β} (h : s.WF) :
+    (s.insert k v).find? x = if k == x then some v else s.find? x := by
+  rw [h.insert.find?_eq, h.find?_eq, BEq.comm,
+    (h.toList'_insert ..).lookup_eq h.insert.nodupKeys, List.lookup]
+  cases eq : x == k <;> simp [eq]
+  induction s.toList' with
+  | nil => rfl
+  | cons kv l ih =>
+    simp [List.filter]; split <;> simp [List.lookup, *]
+    split <;> [skip; rfl]
+    rename_i h1 _ h2
+    simp at h1; simp [h1] at h2; simp [h1, h2] at eq
