Lean4Lean/Std/SMap.lean
@@ -1,0 +1,73 @@
+import Lean.Data.SMap
+import Std.Data.HashMap.Lemmas
+import Lean4Lean.Std.HashMap
+import Lean4Lean.Std.PersistentHashMap
+
+namespace Lean.SMap
+
+variable [BEq α] [Hashable α]
+structure WF (s : SMap α β) where
+  map₂ : s.map₂.WF
+  stage : s.stage₁ → s.map₂ = .empty
+  disjoint : s.map₂.contains a → ¬a ∈ s.map₁
+
+theorem WF.empty : WF ({} : SMap α β) := ⟨.empty, fun _ => rfl, by simp⟩
+
+protected nonrec theorem WF.insert [LawfulBEq α] [LawfulHashable α] {s : SMap α β}
+    (h : s.WF) (k : α) (v : β) (hn : s.find? k = none) : (s.insert k v).WF := by
+  unfold insert; split
+  · refine ⟨h.map₂, h.stage, fun _ h' => ?_⟩
+    have := h.stage
+    simp_all [find?, PersistentHashMap.find?_isSome, PersistentHashMap.WF.empty.find?_eq]
+  · refine ⟨h.map₂.insert .., nofun, fun h1 => ?_⟩
+    simp_all [PersistentHashMap.find?_isSome, h.map₂.find?_insert]
+    revert ‹_›; split
+    · simp_all [find?]
+    · exact h.disjoint ∘ by simp [PersistentHashMap.find?_isSome]
+
+variable [LawfulBEq α] [LawfulHashable α] in
+theorem WF.find?_insert {s : SMap α β} (h : s.WF) :
+    (s.insert k v).find? x = if k == x then some v else s.find? x := by
+  unfold insert; split <;> simp [find?]
+  · exact Std.HashMap.getElem?_insert (α := α)
+  · rw [h.map₂.find?_insert]; split <;> rfl
+
+noncomputable def toList' [BEq α] [Hashable α] (m : SMap α β) :
+    List (α × β) := m.map₂.toList' ++ m.map₁.toList
+
+open scoped _root_.List in
+theorem WF.toList'_insert {α β} [BEq α] [LawfulBEq α] [Hashable α] [LawfulHashable α]
+    {m : SMap α β} (wf : WF m) (a : α) (b : β)
+    (h : m.find? a = none) :
+    (m.insert a b).toList' ~ (a, b) :: m.toList' := by
+  unfold insert; split <;> simp [toList']
+  · have : EquivBEq α := inferInstance; clear ‹LawfulBEq _›
+    have := wf.stage rfl; simp [find?] at this h; subst this; simp
+    refine (List.filter_eq_self.2 ?_ ▸ Std.HashMap.insert_toList (α := α) .. :)
+    rintro ⟨a', b⟩ h
+    refine Decidable.by_contra fun h2 => ?_
+    simp at h2
+    have := Std.HashMap.get?_eq_some_iff_exists_beq_and_mem_toList.2 ⟨_, h2, h⟩
+    exact ‹¬_› (Std.HashMap.mem_of_getElem? this)
+  · refine .append_right (l₂ := _::_) _ ?_
+    refine (List.filter_eq_self.2 ?_ ▸ wf.map₂.toList'_insert .. :)
+    rintro ⟨a', b⟩ h'
+    have := wf.map₂.find?_eq a
+    simp_all [find?]; rintro rfl
+    exact h.1 _ _ h' rfl
+
+theorem WF.find?_eq {α β} [BEq α] [Hashable α] [LawfulBEq α] [LawfulHashable α]
+    {m : SMap α β} (wf : WF m) (a : α) : m.find? a = m.toList'.lookup a := by
+  simp [find?]; split
+  · cases wf.stage rfl
+    simp [toList']
+    exact Std.HashMap.getElem?_eq_lookup_toList ..
+  · simp [toList', List.lookup_append, wf.map₂.find?_eq]
+    cases List.lookup a .. <;> simp [Option.orElse, Std.HashMap.getElem?_eq_lookup_toList]
+
+theorem WF.find?'_eq_find? {α β} [BEq α] [Hashable α] [LawfulBEq α] [LawfulHashable α]
+    {m : SMap α β} (wf : WF m) (a : α) : m.find?' a = m.find? a := by
+  simp [find?, find?']; split; · rfl
+  rename_i m₁ m₂
+  cases e1 : m₁[a]? <;> cases e2 : m₂.find? a <;> simp [Option.orElse]
+  cases wf.disjoint (by simp [PersistentHashMap.find?_isSome, e2]) (Std.HashMap.mem_of_getElem? e1)
