Lean4Lean/Theory/Quot.lean
@@ -6,8 +6,8 @@ namespace Lean4Lean
 def eqConst := vconst(type_of% @Eq)
 def quotConst := vconst(type_of% @Quot)
 def quotMkConst := vconst(type_of% @Quot.mk)
-def quotIndConst := vconst(type_of% @Quot.ind)
 def quotLiftConst := vconst(type_of% @Quot.lift)
+def quotIndConst := vconst(type_of% @Quot.ind)
 def quotDefEq := vdefeq(α r β f c a => @Quot.lift α r β f c (Quot.mk r a) ≡ f a)
 
 def VEnv.QuotReady (env : VEnv) : Prop :=
@@ -16,6 +16,6 @@ def VEnv.QuotReady (env : VEnv) : Prop :=
 def VEnv.addQuot (env : VEnv) : Option VEnv := do
   let env ← env.addConst ``Quot quotConst
   let env ← env.addConst ``Quot.mk quotMkConst
-  let env ← env.addConst ``Quot.ind quotIndConst
   let env ← env.addConst ``Quot.lift quotLiftConst
+  let env ← env.addConst ``Quot.ind quotIndConst
   env.addDefEq quotDefEq
