Lean4Lean/Theory/Typing/QuotLemmas.lean
@@ -9,15 +9,15 @@ theorem addQuot_WF (henv : Ordered env) (hq : QuotReady env) :
   refine with_addConst (cis := [.const _ eqConst]) (hcis := ⟨hq, ⟨⟩⟩) henv
     (fun _ => ⟨_, by type_tac⟩) fun henv => ?_
   refine with_addConst henv (fun ⟨quot, _⟩ => ⟨_, by type_tac⟩) fun henv => ?_
-  refine with_addConst henv (fun ⟨_, quot, _⟩ => ⟨_, by type_tac⟩) fun henv => ?_
-  refine with_addConst henv (fun ⟨_, _, quot, eq, _⟩ => ⟨_, by type_tac⟩) fun henv => ?_
+  refine with_addConst henv (fun ⟨_, quot, eq, _⟩ => ⟨_, by type_tac⟩) fun henv => ?_
+  refine with_addConst henv (fun ⟨_, _, quot, _⟩ => ⟨_, by type_tac⟩) fun henv => ?_
   rintro ⟨_, _, _, _, eq, _⟩ ⟨⟩; exact .defeq henv ⟨by type_tac, by type_tac⟩
 
 section
 variable (henv : addQuot env = some env') include henv
 
-theorem addQuot_objs : env'.HasObjects [.defeq quotDefEq, .const `Quot.lift quotLiftConst,
-    .const `Quot.ind quotIndConst, .const `Quot.mk quotMkConst, .const `Quot quotConst] := by
+theorem addQuot_objs : env'.HasObjects [.defeq quotDefEq, .const `Quot.ind quotIndConst,
+    .const `Quot.lift quotLiftConst, .const `Quot.mk quotMkConst, .const `Quot quotConst] := by
   let ⟨env, h, henv⟩ := HasObjects.bind_const (ls := []) trivial henv
   let ⟨env, h, henv⟩ := HasObjects.bind_const h henv
   let ⟨env, h, henv⟩ := HasObjects.bind_const h henv
@@ -26,8 +26,8 @@ theorem addQuot_objs : env'.HasObjects [.defeq quotDefEq, .const `Quot.lift quot
 
 theorem addQuot_quot : env'.constants ``Quot = quotConst := (addQuot_objs henv).2.2.2.2.1
 theorem addQuot_quotMk : env'.constants ``Quot.mk = quotMkConst := (addQuot_objs henv).2.2.2.1
-theorem addQuot_quotInd : env'.constants ``Quot.ind = quotIndConst := (addQuot_objs henv).2.2.1
-theorem addQuot_quotLift : env'.constants ``Quot.lift = quotLiftConst := (addQuot_objs henv).2.1
+theorem addQuot_quotLift : env'.constants ``Quot.lift = quotLiftConst := (addQuot_objs henv).2.2.1
+theorem addQuot_quotInd : env'.constants ``Quot.ind = quotIndConst := (addQuot_objs henv).2.1
 theorem addQuot_defeq : env'.defeqs quotDefEq := (addQuot_objs henv).1
 
 end
