Lean4Lean/Verify/TypeChecker/Basic.lean
@@ -1,3 +1,0 @@
-import Lean4Lean.Verify.Environment
-
-namespace Lean4Lean
